Pending

proof/correctness/avx2/KyberINDCPA_avx2.ec
@@ -1,13 +1,43 @@
 require import AllCore IntDiv List.
 from Jasmin require import JModel.
-require import Array32 Array128 Array960 Array1088.
+require import Array32 Array128 Array768 Array960 Array1088 Array2304.
 require import KyberPoly  KyberPolyVec KyberINDCPA.
+require import KyberPoly_avx2_proof.
+require import KyberPolyvec_avx2_proof.
 require import Jkem_avx2 Jkem.
 
 import Kyber.
 import KyberSpec.
 import KyberPoly.
 import KyberPolyVec.
+import KyberPolyvecAVX.
+
+equiv sha3equiv :
+ Jkem_avx2.M._sha3_512_32 ~ M._sha3512_32 : ={arg} ==> ={res}.
+admitted. 
+
+op unpackm(v : 'a Array2304.t) = 
+   Array2304.init (fun i =>
+      if 0 <= i < 768 
+      then (unpackv (subarray768 v 0)).[i]
+      else if 768 <= i < 2*768
+           then (unpackv (subarray768 v 1)).[i-768]
+           else (unpackv (subarray768 v 2)).[i-2*768]).
+
+op packm(v : 'a Array2304.t) = 
+   Array2304.init (fun i =>
+      if 0 <= i < 768 
+      then (packv (subarray768 v 0)).[i]
+      else if 768 <= i < 2*768
+           then (packv (subarray768 v 1)).[i-768]
+           else (packv (subarray768 v 2)).[i-2*768]).
+
+
+equiv genmatrixequiv b :
+  Jkem_avx2.M.__gen_matrix ~  M.__gen_matrix :
+    arg{1}.`1 = arg{2}.`1 /\ arg{1}.`2 = b2i b /\ arg{2}.`2 =  W64.of_int (b2i b) ==>
+    res{2} = unpackm res{1}.
+admitted.
 
 lemma kyber_correct_kg_avx2 mem _pkp _skp _randomnessp : 
    equiv [ Jkem_avx2.M.__indcpa_keypair ~ Kyber(KHS,XOF,KPRF,H).kg_derand : 
@@ -45,10 +75,263 @@ transitivity {1} { Jkem.M.__indcpa_keypair(pkp, skp, randomnessp);}
         rho = load_array32 Glob.mem{1} (_pkp + 1152)); 1,2: smt(); 
    last by call(kyber_correct_kg mem _pkp _skp _randomnessp); auto => />. 
 
-inline{1} 1; inline {2} 1.
-sim.
+inline{1} 1; inline {2} 1. sim. 
 
-admitted. (* We should change the axv2 indcpa file to remove useless differences to the ref *)
+call KyberPolyvecAVX.polyvec_tobytes_corr.
+call KyberPolyvecAVX.polyvec_tobytes_corr.
+wp;conseq />.
+ecall (KyberPolyvecAVX.polyvec_reduce_corr (lift_array768 pkpv{1})).
+
+have H := KyberPolyvecAVX.polyvec_add2_corr 2 2 _ _ => //.
+ecall (H (lift_array768 pkpv{1}) (lift_array768 e{1})); clear H.
+unroll for {1} 37.
+
+sp 3 3.
+
+seq 17 17  : (#pre /\ ={publicseed, noiseseed}); 1:  by conseq />; sim;  call( sha3equiv); conseq />; sim. 
+
+seq 1 2 : (#pre /\ a{2} = unpackm aa{1}); 1: by 
+   conseq />; call (genmatrixequiv false); auto => />.
+
+swap {1} [11..12] 2.
+
+seq 10 18 : (#pre /\ ={skpv,e}); 1: by admit. (* to do *)
+
+swap {2} [7..8] -5.
+seq 2 3 : (#pre /\ a{2} = lift_matrix a{1} /\
+            pos_bound2304_cxq a{1} 0 2304 2).
++ inline AuxKyber.__gen_matrix; conseq />.
+  seq 6 3 : (a0{1}=a{2}); last by auto => />;  smt(matrix_unlift).
+  while (i0{1} = i{2} /\ 0<=i0{1}<=kvec /\ seed0{1}=rho{2} /\ !trans{1} /\
+         forall ii jj, 0<=ii<i0{1} => 0<= jj <3 => a0{1}.[ii,jj] = a{2}.[ii,jj]); last  first.
+          auto => />; smt(eq_matrixP).
+  wp; while (i0{1} = i{2} /\ j{1} = j{2} /\ 0<=i0{1}<kvec /\ 0<=j{1}<=kvec /\ seed0{1}=rho{2} /\ !trans{1} /\
+         (forall ii jj, 0<=ii<i0{1} => 0<= jj <3 => a0{1}.[ii,jj] = a{2}.[ii,jj]) /\
+         (forall jj, 0 <= jj <j{1} => a0{1}.[i0{1},jj] = a{2}.[i0{1},jj])); last 
+            by auto => />  /#.
+  wp; call(_: ={XOF.state}); 1: by sim.
+  wp; call(_: ={arg} ==> ={XOF.state}); last by auto => /> &1 &2;  smt(offunmK). 
+  by sim.
+  
+swap {2} [5..9]  -2.
+swap {1} 1 1.
+seq 1 7 : (#pre /\ s{2} = lift_vector skpv{1} /\ e{2} = lift_vector e{1} /\
+                signed_bound768_cxq skpv{1} 0 768 1 /\
+                signed_bound768_cxq e{1} 0 768 1).
++ inline AuxKyber.sample_noise2_spec; conseq />. 
+  seq 8 7 : (noise1{1}=s{2} /\ noise2{1} = e{2}); 1: by sim; auto => />.
+  by auto => />;  smt(vector_unlift).
+
+swap {1} 1 2; seq 0 2: #pre; 1: by auto.
+
+seq 11 3 : (#{/~signed_bound768_cxq skpv{1} 0 768 1}
+             {~signed_bound768_cxq e{1} 0 768 1}pre /\ 
+                t{2} = lift_vector pkpv{1} /\
+                pos_bound768_cxq pkpv{1} 0 768 2 /\
+                pos_bound768_cxq skpv{1} 0 768 2
+                ); last first.
+
++ while{1} (0<=i{1} <= _aux{1} /\ _aux{1} = 4 /\
+            to_uint pkp0{1} = _pkp + 3*384 + i{1} * 8 /\ 
+            to_uint skp0{1} = _skp /\ rho{2} = publicseed{1} /\
+            valid_disj_reg _pkp (384 * 3 + 32) _skp (384 * 3) /\
+            touches2 Glob.mem{1} mem _pkp (384 * 3 + 32) _skp (384 * 3) /\
+                sv{2} = load_array1152 Glob.mem{1} _skp /\
+                tv{2} = load_array1152 Glob.mem{1} _pkp /\ 
+                forall k, 0<=k<i{1}*8 =>
+                 rho{2}.[k] = loadW8 Glob.mem{1} (_pkp + 1152 + k)) 
+             (4 - i{1}).
+
++ move => *;
+  auto => /> &hr ??; rewrite /loadW8 /storeW8 /valid_disj_reg /valid_ptr /=.
+  move  => ppk [#] reg1 reg2 reg3 reg4 reg5 touches2 loaded enter.
+  rewrite to_uintD_small /= 1:/#.
+  do split; 1..3,8:smt().
+  + by rewrite /touches2 /= => a ab1 ab2; rewrite /storeW64 /= /stores /=  !get_set_neqE_s /#.
+  + rewrite /load_array1152 Array1152.tP => k kb.
+    by rewrite !initiE //= /storeW64 /= /stores /=  !get_set_neqE_s /#.
+  + rewrite /load_array1152 Array1152.tP => k kb.
+    by rewrite !initiE //=/storeW64 /= /stores /=  !get_set_neqE_s /#.
+  move => k kbl kbh.
+  case (k <i{hr} * 8).
+  + by move => *;rewrite /storeW64 /= /stores /=  !get_set_neqE_s /#.
+  move => *.  rewrite /storeW64 /= /stores /=.
+  rewrite !get64E !pack8bE // !initiE //= /init8 !initiE 1..8: /#. 
+  by smt(get_set_neqE_s get_set_eqE_s).
+
+  swap {2} 2 -1.
+  wp; ecall(polyvec_tobytes_corr Glob.mem{1} (to_uint pkp{1}) (lift_array768 pkpv{1})). 
+  wp; ecall(polyvec_tobytes_corr Glob.mem{1} (to_uint skp{1}) (lift_array768 skpv{1})).
+  auto => /> &1 &2 *.
+  do split.
+  + move => *. rewrite /lift_vector /toipolyvec /fromarray256 !mapiE //. 
+    by smt(rg_asint).
+  + move => *. rewrite /lift_vector /toipolyvec /fromarray256 /lift_array768 tP => k kb.  
+    rewrite !mapiE // asintK /=.  
+    rewrite !offunvE //= /lift_array256 /subarray256 initiE //=. 
+    case (0 <= k && k < 256); 1: by move => *; rewrite mapiE //= initiE //.
+    case (256 <= k && k < 512); 1: by  move => *; rewrite mapiE 1:/# /= initiE /#.
+    by  move => *; rewrite mapiE 1:/# /= initiE /#.
+
+  move => ???; rewrite /touches => touches0.
+  do split.
+  + move => *. rewrite /lift_vector /toipolyvec /fromarray256 !mapiE //. 
+    by smt(rg_asint).
+  + move => *. rewrite /lift_vector /toipolyvec /fromarray256 /lift_array768 tP => k kb.  
+    rewrite !mapiE // asintK /=.  
+    rewrite !offunvE //= /lift_array256 /subarray256 initiE //=. 
+    case (0 <= k && k < 256); 1: by move => *; rewrite mapiE //= initiE //.
+    case (256 <= k && k < 512); 1: by  move => *; rewrite mapiE 1:/# /= initiE /#.
+    by  move => *; rewrite mapiE 1:/# /= initiE /#.
+  + by smt().
+
+  move => ?????; rewrite /touches => touches1.
+  do split => //.
+  + by rewrite to_uintD_small //=. 
+  + rewrite /touches2 /= => a ab1 ab2. 
+    have ? := (touches1 (a - to_uint pkp{1}) _); 1: by smt().
+    by have ? := (touches0 (a - to_uint skp{1}) _); by smt().
+  + rewrite /load_array1152 tP => k kb; rewrite !initiE //=. 
+    move : (touches1 (to_uint skp{1} - to_uint pkp{1} + k) _); 1: by smt().
+    by have -> ->: to_uint pkp{1} + (to_uint skp{1} - to_uint pkp{1} + k) = to_uint skp{1} + k by ring.
+  + by smt().
+  
+  move => * /=.
+  split; 1: by smt(). 
+  by move => *;rewrite /load_array32 tP => k kb; rewrite initiE //= /#. 
+
+(* Algebraic part remaining *)
+conseq => />.
+
+seq 1 1 : (#{/~signed_bound768_cxq skpv{1} 0 768 1}pre /\
+            pos_bound768_cxq skpv{1} 0 768 2).
++ wp;ecall{1} (polyvec_ntt_corr (skpv{1})).
+  by auto => /> /#.
+
+seq 1 1 : (#{/~signed_bound768_cxq e{1} 0 768 1}pre /\
+            pos_bound768_cxq e{1} 0 768 2).
++ wp;ecall{1} (polyvec_ntt_corr (e{1})).
+  by auto => /> /#.
+
+seq 3 0 : (#pre /\
+    forall k, 0 <= k < 256 =>
+         b16 pkpv{1}.[k]  (2*q)  /\ 
+    inFq (to_sint pkpv{1}.[k]) = (ntt_mmul a{2} s{2}).[0].[k]).
+
+wp; ecall{1} (innerprod_corr 
+     (invnttv (lift_vector (Array768.init (fun (i_0 : int) => a{1}.[0 + i_0]))))
+     (invnttv (lift_vector skpv{1}))).
+
++ auto => /> &1 &2.
+  move => ???????.
+  do split; 1,2,4: smt(nttvK).
+  + by rewrite /signed_bound768_cxq => k kb; rewrite initiE //= /#.
+  move => ????result0; rewrite /lift_matrix.
+  rewrite /lift_array2304 /lift_vector /lift_array256  !tP =>  ?val k kbl kbh.
+  rewrite !initiE 1:/# /= kbl kbh /= ; do split; 1,2:smt().
+  move : (val k _) => //; rewrite mapiE //= => ->.
+  rewrite /ntt_mmul offunvE //= /dotp /kvec /=.
+  rewrite !Big.BAdd.big_consT //= !Big.BAdd.big_nil //=. 
+  rewrite !offunvE //= !offunvK /vclamp !offunmE //= /kvec /=.
+  rewrite !add_comm_ntt !mul_comm_ntt !nttK nttZero. 
+  rewrite -!(matrixcols) //.
+
+seq 2 0 : (#pre /\
+        (forall k, 256 <= k < 512 =>
+         b16 pkpv{1}.[k]  (2*q)  /\ 
+    inFq (to_sint pkpv{1}.[k]) = (ntt_mmul a{2} s{2}).[1].[k-256])
+).
+
+wp; ecall{1} (innerprod_corr 
+     (invnttv (lift_vector (Array768.init (fun (i_0 : int) => a{1}.[768 + i_0]))))
+     (invnttv (lift_vector skpv{1}))).
+
++ auto => /> &1 &2.
+  move => ????????.
+  do split; 1,2,4: smt(nttvK).
+  + by rewrite /signed_bound768_cxq => k kb; rewrite initiE //= /#.
+  move => ????result0; rewrite /lift_matrix.
+  rewrite /lift_array2304 /lift_vector /lift_array256  !tP =>  ?val.
+  split.
+  + move => k klb khb; rewrite !initiE 1:/# /=; do split; 1,2:smt().
+    by rewrite (_: !(256 <= k && k < 512)) /# /=.
+  move => k kbl kbh;rewrite !initiE 1:/# /= kbl kbh /= ; do split; 1,2:smt().
+  move : (val (k-256) _);1:smt(); rewrite mapiE 1:/# => ->.
+  rewrite /ntt_mmul offunvE //= /dotp /kvec /=.
+  rewrite !Big.BAdd.big_consT //= !Big.BAdd.big_nil //=. 
+  rewrite !offunvE //= !offunvK /vclamp !offunmE //= /kvec /=.
+  rewrite !add_comm_ntt !mul_comm_ntt !nttK nttZero. 
+  by rewrite -!(matrixcols) //.
+
+seq 2 0 : (#pre /\
+        (forall k, 512 <= k < 768 =>
+         b16 pkpv{1}.[k]  (2*q)  /\ 
+    inFq (to_sint pkpv{1}.[k]) = (ntt_mmul a{2} s{2}).[2].[k-512])
+).
+
+wp; ecall{1} (innerprod_corr 
+     (invnttv (lift_vector (Array768.init (fun (i_0 : int) => a{1}.[2*768 + i_0]))))
+     (invnttv (lift_vector skpv{1}))).
+
++ auto => /> &1 &2.
+  move => ?????????.
+  do split; 1,2,4: smt(nttvK).
+  + by rewrite /signed_bound768_cxq => k kb; rewrite initiE //= /#.
+  move => ????result0; rewrite /lift_matrix.
+  rewrite /lift_array2304 /lift_vector /lift_array256  !tP =>  ?val.
+  do split.
+  + move => k klb khb; rewrite !initiE 1:/# /=; do split; 1,2:smt().
+    by rewrite (_: !(512 <= k && k < 768)) /# /=.
+  + move => k klb khb; rewrite !initiE 1:/# /=; do split; 1,2:smt().
+    by rewrite (_: !(512 <= k && k < 768)) /# /=.
+  move => k kbl kbh;rewrite !initiE 1:/# /= kbl kbh /= ; do split; 1,2:smt().
+  move : (val (k-512) _);1:smt(); rewrite mapiE 1:/# => ->.
+  rewrite /ntt_mmul offunvE //= /dotp /kvec /=.
+  rewrite !Big.BAdd.big_consT //= !Big.BAdd.big_nil //=. 
+  rewrite !offunvE //= !offunvK /vclamp !offunmE //= /kvec /=.
+  rewrite !add_comm_ntt !mul_comm_ntt !nttK nttZero. 
+  by rewrite -!(matrixcols) //.
+
+conseq => />.
+
+seq 1 1 : (t{2} = lift_vector pkpv{1} /\ signed_bound768_cxq pkpv{1} 0 768 4);
+last first.
+
++ ecall {1} (polyvec_reduce_corr (lift_array768 pkpv{1})).
+  auto => /> // &1 ?; rewrite /lift_array768 =>  rr  rrv ?. 
+  rewrite /lift_vector eq_vectorP => i ib; rewrite !offunvE//=.
+  rewrite /lift_array256 /subarray256 tP => k kb.
+  rewrite !mapiE //= !initiE //=.
+  move : rrv; rewrite tP => rrv.
+  move : (rrv (256 * i + k) _); 1: smt().
+  by rewrite !mapiE 1,2:/# /=. 
+
+have H := polyvec_add_corr_impl 2 2 _ _ => //.
+ecall{1} (H (lift_array768 pkpv{1}) (lift_array768 e{1})).
+clear H.
+auto => /> &1 &2 ??????? vs0 vs1 vs2.
+
+do split; 1,2:smt().
+
+move => ?? resf ? vsf; rewrite eq_vectorP => r rb.
+rewrite /(lift_vector resf) !offunvE //= /lift_array256 tP => k kb.
+rewrite mapiE //= /subarray256 initiE //= /(&+) map2E /=.
+rewrite /(lift_vector e{1}) !offunvE //=.
+case(r = 0).
++ move => r0; rewrite r0 /= vsf 1:/# /= initiE //= subliftsub //=; congr.
+  rewrite /lift_array768 mapiE 1:/# /=;move : (vs0 k _); 1: by smt().
+  by move => [#] _ _ ->; rewrite /ntt_mmul offunvE //=.
+
+case(r = 1).
++ move => r1 nr0; rewrite r1 /= vsf 1:/# /= initiE //= subliftsub //=; congr.
+  rewrite /lift_array768 mapiE 1:/# /=;move : (vs1 (256 + k) _); 1: by smt().
+  by move => [#] _ _ ->; rewrite /ntt_mmul offunvE //=.
+
+case(r = 2); last by smt().
+move => r2 nr1 nr0; rewrite r2 /= vsf 1:/# /= initiE //= subliftsub //=; congr.
+rewrite /lift_array768 mapiE 1:/# /=;move : (vs2 (512 + k) _); 1: by smt().
+by move => [#] _ _ ->; rewrite /ntt_mmul offunvE //=.
+qed.
 
 
 
