proof/correctness/avx2/KyberPolyvec_avx2_proof.ec
@@ -3,11 +3,12 @@ from Jasmin require import JModel.
 require import Fq Array16 Array32 Array128 Array256 Array400 Array768.
 require import W16extra WArray32 WArray256 WArray512 WArray800 WArray1536 WArray168 WArray800.
 require import AVX2_Ops.
-require import Jkem_avx2.
+require import Jkem_avx2 Jkem.
 require import KyberPolyvec_avx2_prevec.
 require import KyberPoly_avx2_proof.
 require import Fq_avx2.
 require import KyberPolyVec.
+require import KyberPolyvec_avx2_vec.
 
 theory KyberPolyvecAVX.
 
@@ -21,8 +22,8 @@ import KyberPoly.
 import KyberPoly.
 
 lemma polvec_add_corr_h _a _b ab bb:
+    0 <= ab <= 6 => 0 <= bb <= 3 =>  
       hoare[Mprevec.polyvec_add2:
-           (0 <= ab <= 6 /\ 0 <= bb <= 3) /\
            _a = lift_array768 r /\
            _b = lift_array768 b /\
            signed_bound768_cxq r 0 768 ab /\
@@ -32,26 +33,26 @@ lemma polvec_add_corr_h _a _b ab bb:
            forall k, 0 <= k < 768 =>
              inFq (to_sint res.[k]) = _a.[k] + _b.[k]].
 proof.
+  move => abb bbb.
   proc.
   wp.
-  admit. (*
-  ecall (KyberPolyAVX.poly_add_corr (lift_array256 (Array256.init (fun i => r.[(2 * 256) + i]))) (lift_array256 (Array256.init (fun i => b.[(2 * 256) + i]))) ab bb).
+  call (KyberPolyAVX.poly_add_corr_h (Array256.init (fun i => _a.[(2 * 256) + i])) (Array256.init (fun i => _b.[(2 * 256) + i])) ab bb abb bbb).
   wp.
-  ecall (KyberPolyAVX.poly_add_corr (lift_array256 (Array256.init (fun i => r.[256 + i]))) (lift_array256 (Array256.init (fun i => b.[256 + i]))) ab bb).
+  call (KyberPolyAVX.poly_add_corr_h (Array256.init (fun i => _a.[256 + i])) (Array256.init (fun i => _b.[256 + i])) ab bb abb bbb).
   wp.
-  ecall (KyberPolyAVX.poly_add_corr (lift_array256 (Array256.init (fun i => r.[0 + i]))) (lift_array256 (Array256.init (fun i => b.[0 + i]))) ab bb).
+  call (KyberPolyAVX.poly_add_corr_h (Array256.init (fun i => _a.[0 + i])) (Array256.init (fun i => _b.[0 + i])) ab bb abb bbb).
   wp. skip.
-  move => &hr [[a_i b_i] [_a_def] [_b_def] [sgnd_bnd_rp] sgnd_bnd_bp].
-  rewrite a_i b_i => />.
+  move => /= &hr; rewrite /lift_array768 /lift_array256 !tP => [#] _a_def _b_def sgnd_bnd_rp sgnd_bnd_bp.
   split.
-  smt(@Array768 @Array256).
-  move => sgnd_bnd_rp_1 sgnd_bnd_bp_1 result_1 sgnd_bnd_res_1 res_1_def.
+  + do split => /=; smt(@Array768 @Array256). 
+    
+  move => [#] ??? sgnd_bnd_bp_1 result_1 [#]  sgnd_bnd_res_1 res_1_def.
   split.
-  smt(@Array256 @Array768).
-  move => sgnd_bnd_rp_2 sgnd_bnd_bp_2 result_2 sgnd_bnd_res_2 res_2_def.
+  + rewrite !tP;do split; move => *; rewrite !initiE; smt(@Array256 @Array768).
+  move => [#] ???sgnd_bnd_bp_2 result_2 [#] sgnd_bnd_res_2 res_2_def.
   split.
-  smt(@Array256 @Array768).
-  move => sgnd_bnd_rp_3 sgnd_bnd_bp_3 result_3 sgnd_bnd_res_3 res_3_def.
+  + rewrite !tP;do split; move => *; rewrite !initiE /= // ?mapiE //; smt(@Array256 @Array768).
+  move => [#] ??? sgnd_bnd_bp_3 result_3 [#] sgnd_bnd_res_3 res_3_def.
   split.
   rewrite /signed_bound768_cxq.
   rewrite /signed_bound_cxq /b16 in sgnd_bnd_res_1.
@@ -61,7 +62,7 @@ proof.
   do rewrite initiE //=.
   move : (sgnd_bnd_res_1 k) (sgnd_bnd_res_2 (k - 256)) (sgnd_bnd_res_3 (k - 512)).
   smt(@Array768 @Array256 @Int).
-  move => k k_lb k_ub.
+  move => k [#] k_lb k_ub.
   do rewrite initiE //=.
   case (0 <= k < 256) => k_si.
   move : (res_1_def k k_si).
@@ -80,12 +81,28 @@ proof.
   rewrite -lezNgt in k_ssi.
   rewrite k_ub k_ssi //=.
   rewrite /lift_array256.
-  do rewrite mapiE 1:/#.
   do rewrite initiE 1:/#.
   smt(@Array256 @Array768 @KyberPolyAVX @Int).
-  *)
 qed.
 
+lemma polyvec_add_ll : islossless Mprevec.polyvec_add2
+  by proc; do 3!(wp; call KyberPolyAVX.poly_add_ll).
+
+lemma polvec_add_corr _a _b ab bb:
+    0 <= ab <= 6 => 0 <= bb <= 3 =>  
+      phoare[Mprevec.polyvec_add2:
+           _a = lift_array768 r /\
+           _b = lift_array768 b /\
+           signed_bound768_cxq r 0 768 ab /\
+           signed_bound768_cxq b 0 768 bb
+           ==>
+           signed_bound768_cxq res 0 768 (ab + bb) /\
+           forall k, 0 <= k < 768 =>
+             inFq (to_sint res.[k]) = _a.[k] + _b.[k]] = 1%r.
+  move => abb bbb.
+  conseq (polyvec_add_ll) (polvec_add_corr_h _a _b ab bb abb bbb).
+  by smt().
+qed.
 
 lemma polyvec_csubq_corr ap :
   hoare[Mprevec.polyvec_csubq:
@@ -103,35 +120,36 @@ proof.
   wp.
   ecall (KyberPolyAVX.poly_csubq_corr_h (lift_array256 (Array256.init (fun (i : int) => r.[i])))).
    wp. skip.
-   move => &hr [ap_def pos_bound_r]; split.
+   rewrite /lift_array768 /lift_array256 /pos_bound256_cxq !tP;move => &hr [ap_def pos_bound_r]; split.
    split; trivial; smt(@Array256).
-   admit.
-(*
    move => [r_eq_r_1 pos_bound_r_1 res1 [r_eq_res_1 pos_bound_res_1] res_1_def]; split.
-   split; trivial; smt(@Array768 @Array256).
+   split; trivial => k kb @/res_1_def; rewrite !initiE //=; smt(@Array768 @Array256 qE).
    move => [r_eq_r_2 pos_bound_r_2 res2 [r_eq_res_2 pos_bound_res_2] res_2_def]; split.
-   split; trivial; smt(@Array768 @Array256).
+   split; trivial => k kb @/res_2_def; rewrite !initiE //=; smt(@Array768 @Array256 qE).
    move => [r_eq_r_3 pos_bound_r_3 res3 [r_eq_res_3 pos_bound_res_3] res_3_def]; split.
    rewrite /res_3_def /res_2_def /res_1_def /=.
-   rewrite ap_def.
-   rewrite lift_array768P; move => k k_i.
+   rewrite tP => k kb; rewrite ap_def // !mapiE //= initiE //=.
+   case (512 <= k < 768) => k_si. 
+   rewrite tP in r_eq_res_3; move : (r_eq_res_3 (k - 512) _);  1:by smt().
+   rewrite !mapiE 1,2:/# /= => <-.
    do rewrite initiE 1:/# //=.
-   do rewrite fun_if.
-   rewrite lift_array256P //= in r_eq_res_3.
-   rewrite lift_array256P //= in r_eq_res_2.
-   rewrite lift_array256P //= in r_eq_res_1.
-   case (512 <= k < 768) => k_si.
-   rewrite -(r_eq_res_3 (k - 512)) 1:/#.
-   do rewrite initiE 1:/# //=.
-   rewrite (_: (256 <= k && k < 512) = false) 1:/# //=.
-   rewrite (_: (0 <= k && k < 256) = false) 1:/# //=.
    case (256 <= k < 512) => k_ssi.
-   rewrite -(r_eq_res_2 (k -  256)) 1:/#.
+   rewrite tP in r_eq_res_2; move : (r_eq_res_2 (k - 256) _);  1:by smt().
+   rewrite !mapiE 1,2:/# /= => <-.
    do rewrite initiE 1:/# //=.
-   rewrite (_: (0 <= k && k < 256) = false) 1:/# //=.
-   rewrite -(r_eq_res_1 k) 1:/#.
+   rewrite tP in r_eq_res_1; move : (r_eq_res_1 (k ) _);  1:by smt().
+   rewrite !mapiE 1,2:/# /=.
    do rewrite initiE 1:/# //=.
-   rewrite /res_3_def /res_2_def /res_1_def.
+    by smt(). by smt().
+   case (256 <= k < 512) => k_ssi.
+   do rewrite initiE 1:/# //= k_ssi /=.
+   rewrite tP in r_eq_res_2; move : (r_eq_res_2 (k - 256) _);  1:by smt().
+   rewrite !mapiE 1,2:/# /= => <-.
+   do rewrite initiE 1:/# //=. smt().
+   rewrite tP in r_eq_res_1; move : (r_eq_res_1 (k ) _);  1:by smt().
+   rewrite !mapiE 1,2:/# /=.
+   do rewrite initiE 1:/# //=.
+    by smt(). 
    rewrite /pos_bound768_cxq => k k_i.
    do rewrite initiE //=.
    rewrite /pos_bound256_cxq /bpos16 //=in pos_bound_res_3.
@@ -139,11 +157,10 @@ proof.
    rewrite /pos_bound256_cxq /bpos16 //=in pos_bound_res_1.
    move : (pos_bound_res_3 (k - 512))  (pos_bound_res_2 (k - 256))  (pos_bound_res_1 k).
    smt(@Array256 @Array768).
-*)
 qed.
 
 
-lemma polyvec_reduce_corr _a:
+lemma polyvec_reduce_corr_h _a:
   hoare[Mprevec.polyvec_reduce:
        _a  = lift_array768 r ==>
        _a  = lift_array768 res /\
@@ -163,25 +180,25 @@ proof.
   split.
   rewrite /res3_def /res2_def /res1_def /=.
   rewrite _a_def.
-  admit. (*
-  rewrite lift_array768P; move => k k_i.
+  rewrite /lift_array768 tP => k kb.
+  rewrite !mapiE //=.
   do rewrite initiE 1:/# //=.
   do rewrite fun_if.
-  rewrite lift_array256P //= in r_eq_res3.
-  rewrite lift_array256P //= in r_eq_res2.
-  rewrite lift_array256P //= in r_eq_res1.  
    case (512 <= k < 768) => k_si.
-   rewrite -(r_eq_res3 (k - 512)) 1:/#.
+   rewrite /lift_array256 tP in r_eq_res3; move : (r_eq_res3 (k - 512) _);  1:by smt().
+   rewrite !mapiE 1,2:/# /= => <-.
    do rewrite initiE 1:/# //=.
-   rewrite (_: (256 <= k && k < 512) = false) 1:/# //=.
-   rewrite (_: (0 <= k && k < 256) = false) 1:/# //=.
    case (256 <= k < 512) => k_ssi.
-   rewrite -(r_eq_res2 (k -  256)) 1:/#.
-   do rewrite initiE 1:/# //=.
-   rewrite (_: (0 <= k && k < 256) = false) 1:/# //=.
-   rewrite -(r_eq_res1 k) 1:/#.
-   do rewrite initiE 1:/# //=.
-   rewrite /res3_def /res2_def /res1_def. *)
+   rewrite /lift_array256 tP in r_eq_res2; move : (r_eq_res2 (k - 256) _);  1:by smt().
+   rewrite !mapiE 1,2:/# /= => <-.
+   do rewrite initiE 1:/# //=. smt(). smt(). 
+   case (256 <= k < 512) => k_ssi.
+   rewrite /lift_array256 tP in r_eq_res2; move : (r_eq_res2 (k - 256) _);  1:by smt().
+   rewrite !mapiE 1,2:/# /= => <-.
+   do rewrite initiE 1:/# //=. smt().  
+   rewrite /lift_array256 tP in r_eq_res1; move : (r_eq_res1 (k) _);  1:by smt().
+   rewrite !mapiE 1,2:/# /= => <-.
+   do rewrite initiE 1:/# //=.   
    move => k k_i.
    do rewrite initiE //=.
    rewrite /bpos16 //=in res3_bound.
@@ -190,6 +207,150 @@ proof.
    move : (res3_bound (k - 512))  (res2_bound (k - 256))  (res1_bound k).
    smt(@Array256 @Array768).
 qed.
+
+lemma polyvec_reduce_ll : islossless Mprevec.polyvec_reduce
+  by proc; do 3!(wp; call KyberPolyAVX.poly_reduce_ll).
+
+lemma polvec_reduce_corr _a:
+      phoare[Mprevec.polyvec_reduce:
+       _a  = lift_array768 r ==>
+       _a  = lift_array768 res /\
+       forall k, 0 <= k < 768 => bpos16 res.[k] (2*q)] = 1%r.
+  conseq (polyvec_reduce_ll) (polyvec_reduce_corr_h _a).
+  by smt().
+qed.
+
+
+abbrev nttpack_idx = Array256.of_list witness
+  [0; 16; 32; 48; 64; 80; 96; 112; 1; 17; 33; 49; 65; 81; 97; 113;
+   2; 18; 34; 50; 66; 82; 98; 114; 3; 19; 35; 51; 67; 83; 99; 115;
+   4; 20; 36; 52; 68; 84; 100; 116; 5; 21; 37; 53; 69; 85; 101; 117;
+   6; 22; 38; 54; 70; 86; 102; 118; 7; 23; 39; 55; 71; 87; 103; 119;
+   8; 24; 40; 56; 72; 88; 104; 120; 9; 25; 41; 57; 73; 89; 105; 121;
+   10; 26; 42; 58; 74; 90; 106; 122; 11; 27; 43; 59; 75; 91; 107; 123;
+   12; 28; 44; 60; 76; 92; 108; 124; 13; 29; 45; 61; 77; 93; 109; 125;
+   14; 30; 46; 62; 78; 94; 110; 126; 15; 31; 47; 63; 79; 95; 111; 127;
+   128; 144; 160; 176; 192; 208; 224; 240; 129; 145; 161; 177; 193; 209; 225; 241;
+   130; 146; 162; 178; 194; 210; 226; 242; 131; 147; 163; 179; 195; 211; 227; 243;
+   132; 148; 164; 180; 196; 212; 228; 244; 133; 149; 165; 181; 197; 213; 229; 245;
+   134; 150; 166; 182; 198; 214; 230; 246; 135; 151; 167; 183; 199; 215; 231; 247;
+   136; 152; 168; 184; 200; 216; 232; 248; 137; 153; 169; 185; 201; 217; 233; 249;
+   138; 154; 170; 186; 202; 218; 234; 250; 139; 155; 171; 187; 203; 219; 235; 251;
+   140; 156; 172; 188; 204; 220; 236; 252; 141; 157; 173; 189; 205; 221; 237; 253;
+   142; 158; 174; 190; 206; 222; 238; 254; 143; 159; 175; 191; 207; 223; 239; 255].
+
+abbrev nttunpack_idx = Array256.of_list witness
+  [0; 8; 16; 24; 32; 40; 48; 56; 64; 72; 80; 88; 96; 104; 112; 120;
+   1; 9; 17; 25; 33; 41; 49; 57; 65; 73; 81; 89; 97; 105; 113; 121;
+   2; 10; 18; 26; 34; 42; 50; 58; 66; 74; 82; 90; 98; 106; 114; 122;
+   3; 11; 19; 27; 35; 43; 51; 59; 67; 75; 83; 91; 99; 107; 115; 123;
+   4; 12; 20; 28; 36; 44; 52; 60; 68; 76; 84; 92; 100; 108; 116; 124;
+   5; 13; 21; 29; 37; 45; 53; 61; 69; 77; 85; 93; 101; 109; 117; 125;
+   6; 14; 22; 30; 38; 46; 54; 62; 70; 78; 86; 94; 102; 110; 118; 126;
+   7; 15; 23; 31; 39; 47; 55; 63; 71; 79; 87; 95; 103; 111; 119; 127;
+   128; 136; 144; 152; 160; 168; 176; 184; 192; 200; 208; 216; 224; 232; 240; 248;
+   129; 137; 145; 153; 161; 169; 177; 185; 193; 201; 209; 217; 225; 233; 241; 249;
+   130; 138; 146; 154; 162; 170; 178; 186; 194; 202; 210; 218; 226; 234; 242; 250;
+   131; 139; 147; 155; 163; 171; 179; 187; 195; 203; 211; 219; 227; 235; 243; 251;
+   132; 140; 148; 156; 164; 172; 180; 188; 196; 204; 212; 220; 228; 236; 244; 252;
+   133; 141; 149; 157; 165; 173; 181; 189; 197; 205; 213; 221; 229; 237; 245; 253;
+   134; 142; 150; 158; 166; 174; 182; 190; 198; 206; 214; 222; 230; 238; 246; 254;
+   135; 143; 151; 159; 167; 175; 183; 191; 199; 207; 215; 223; 231; 239; 247; 255].
+
+
+op unpack(a : 'a Array256.t) = 
+    Array256.init (fun i => a.[nttunpack_idx.[i]]).
+
+op pack(a : 'a Array256.t) = 
+    Array256.init (fun i => a.[nttpack_idx.[i]]).
+
+lemma packK : cancel pack<:'a> unpack<:'a>
+  by rewrite /cancel => x; apply Array256.all_eq_eq => @/unpack @/pack @/all_eq/=.
+
+lemma unpackK : cancel unpack<:'a> pack<:'a>
+  by rewrite /cancel => x; apply Array256.all_eq_eq => @/unpack @/pack @/all_eq/=.
+
+op unpackv(v : 'a Array768.t) = 
+   Array768.init (fun i =>
+      if 0 <= i < 256 
+      then (unpack (subarray256 v 0)).[i]
+      else if 256 <= i < 512
+           then (unpack (subarray256 v 1)).[i-256]
+           else (unpack (subarray256 v 2)).[i-512]).
+
+op packv(v : 'a Array768.t) = 
+   Array768.init (fun i =>
+      if 0 <= i < 256 
+      then (pack (subarray256 v 0)).[i]
+      else if 256 <= i < 512
+           then (pack (subarray256 v 1)).[i-256]
+           else (pack (subarray256 v 2)).[i-512]).
+
+
+lemma polyvec_tobytes_corr :
+    equiv [ Jkem_avx2.M.__polyvec_tobytes ~ Jkem.M.__polyvec_tobytes :
+             pos_bound768_cxq a{1} 0 256 2 /\
+             pos_bound768_cxq a{2} 0 256 2 /\
+             lift_array768 a{1} = lift_array768 (unpackv a{2}) /\ ={rp,Glob.mem} ==> ={Glob.mem} ].
+admitted.
+
+lemma polyvec_add2_corr  (ab bb : int):
+    0 <= ab && ab <= 6 =>
+    0 <= bb && bb <= 3 =>
+  forall (_a _b : Fq Array768.t),
+    equiv [ Jkem_avx2.M.__polyvec_add2 ~ Jkem.M.__polyvec_add2 :
+      _a = lift_array768 r{2} /\
+      _b = lift_array768 b{2} /\ signed_bound768_cxq r{2} 0 768 ab /\ signed_bound768_cxq b{2} 0 768 bb /\
+      _a = lift_array768 (packv r{1}) /\
+      _b = lift_array768 (packv b{1}) /\ signed_bound768_cxq r{1} 0 768 ab /\ signed_bound768_cxq b{1} 0 768 bb
+           ==> lift_array768 res{1} = lift_array768  (unpackv res{2}) /\
+               signed_bound768_cxq res{1} 0 768 (ab + bb) /\
+               signed_bound768_cxq res{2} 0 768 (ab + bb) 
+              ].
+proof. 
+move => abb bbb _a _b;proc* => /=.
+transitivity {1} {r0 <@ Mprevec.polyvec_add2(r,b); }
+       (={r,b} ==> ={r0})
+       (_a = lift_array768 r{2} /\
+  _b = lift_array768 b{2} /\
+  signed_bound768_cxq r{2} 0 768 ab /\
+  signed_bound768_cxq b{2} 0 768 bb /\
+  _a = lift_array768 (packv r{1}) /\
+  _b = lift_array768 (packv b{1}) /\ signed_bound768_cxq r{1} 0 768 ab /\ signed_bound768_cxq b{1} 0 768 bb   ==> 
+      lift_array768 r0{1} = lift_array768  (unpackv r0{2}) /\ signed_bound768_cxq r0{1} 0 768 (ab + bb) /\ signed_bound768_cxq r0{2} 0 768 (ab + bb)); 1,2: by smt().
+  + symmetry. call prevec_eq_poly_add2 => //.
+have corr1 := (polvec_add_corr (unpackv _a) (unpackv _b) ab bb abb bbb). call {1} corr1.
+have corr2 := (polyvec_add_corr _a _b ab bb abb bbb); call {2} corr2.
+
+auto => />. 
+move => &1 &2 ????->->?????; do split. admit. admit.
+move => *.
+admit.
+qed.
+
+lemma polyvec_reduce_corr _a :
+    equiv [ Jkem_avx2.M.__polyvec_reduce ~ Jkem.M.__polyvec_reduce :
+       _a  = lift_array768 r{2} /\  _a  = lift_array768 (packv r{1})  ==>
+       (forall k, 0 <= k < 768 => bpos16 res{1}.[k] (2*q)) /\
+       (forall k, 0 <= k < 768 => bpos16 res{2}.[k] (2*q)) /\
+              lift_array768 res{1} = lift_array768 (unpackv res{2}) ].
+proc*. 
+transitivity {1} {r0 <@ Mprevec.polyvec_reduce(r); }
+       (={r} ==> ={r0})
+       (_a = lift_array768 r{2} /\ _a = lift_array768 (packv r{1})   ==> 
+      (forall (k : int), 0 <= k && k < 768 => bpos16 r0{1}.[k] (2 * q)) /\
+  (forall (k : int), 0 <= k && k < 768 => bpos16 r0{2}.[k] (2 * q)) /\
+  lift_array768 r0{1} = lift_array768 (unpackv r0{2})); 1,2: by smt().
+  + symmetry. call prevec_eq_poly_reduce => //.
+have corr1 := (polvec_reduce_corr (unpackv _a)). call {1} corr1.
+have corr2 := (polyvec_reduce_corr _a); call {2} corr2.
+
+auto => />. 
+move => &1 &2 ???->?; do split. admit. 
+move => ??<-?.
+admit.
+qed.
+
 
 end KyberPolyvecAVX.
 
